reorganized; working on a reflective tactic

dpll.v
@@ -1,189 +1,13 @@
 Set Implicit Arguments.
-Require Import List Arith.
+Require Import List Arith Omega.
 
 (*=============================================================================
- * sublist
- *===========================================================================*)
-
-Section sublist.
-
-  Ltac e := eauto 3 with list.
-
-  Local Hint Constructors Forall : list.
-  Local Hint Resolve in_or_app Forall_impl : list.
-
-  Variable A : Type.
-
-  Definition sublist (x y : list A) := List.Forall (fun a => In a y) x.
-
-  Lemma sublist_refl : forall (x : list A), sublist x x.
-    unfold sublist; induction x; e.
-    constructor; simpl; e.
-    eapply Forall_impl; try eassumption; e.
-  Qed.
-
-  Lemma sublist_app : forall (l x y : list A), sublist l x \/ sublist l y
-                                                 -> sublist l (x ++ y).
-    induction l.
-    {
-      unfold sublist; simpl; intros; e.
-    }
-    {
-      unfold sublist; simpl; intros.
-      constructor.
-      destruct H; inversion_clear H; e.
-      apply IHl.
-      destruct H; inversion_clear H; e.
-    }
-  Qed.
-
-  Lemma sublist_In : forall x (a : A) y, sublist x y -> In a x -> In a y.
-    induction x; simpl; try tauto; inversion_clear 1; destruct 1; subst; auto.
-  Qed.
-
-End sublist.
-
-Local Hint Resolve sublist_refl sublist_app sublist_In.
-
-
-(*=============================================================================
- * formulas and their interpretations
+ * dpll
  *===========================================================================*)
 
 Inductive lit := pos : nat -> lit | neg : nat -> lit.
 Definition clause := list lit.
 Definition formula := list clause.
-
-Definition interp := nat -> bool.
-
-Definition interpLit (I : interp) (l : lit) :=
-  match l with
-    | pos n => I n
-    | neg n => negb (I n)
-  end.
-
-Definition interpClause (I : interp) (c : clause) :=
-  fold_right (fun l b => orb (interpLit I l) b) false c.
-
-Definition interpFormula (I : interp) (f : formula) :=
-  fold_right (fun c b => andb (interpClause I c) b) true f.
-
-Definition satisfiable f := exists i, interpFormula i f = true.
-
-Definition entails f c := forall i, interpFormula i f = true
-                                    -> interpClause i c = true.
-
-
-(*=============================================================================
- * tests
- *===========================================================================*)
-
-Example I n := match n with 0 => false | 1 => true | _ => true end.
-Eval simpl in interpLit I (pos 0).
-
-Goal forall (i : interp), interpClause i nil = false.
-  simpl; auto.
-Qed.
-
-Goal forall (i : interp), interpFormula i nil = true.
-  simpl; auto.
-Qed.
-
-Goal forall (i : interp) v, interpClause i ((pos v) :: (neg v) :: nil) = true.
-  simpl; intros.
-  destruct (i v) eqn:?; simpl; auto.
-Qed.
-
-Example c1 := pos 3 :: nil.
-Example c2 := neg 3 :: nil.
-
-Goal forall (i : interp), interpFormula i (c1 :: c2 :: nil) = false.
-  simpl; intros.
-  destruct (i 3) eqn:?; simpl; auto.
-Qed.
-
-
-(*=============================================================================
- * interp facts
- *===========================================================================*)
-
-Lemma interpClause_exists : forall i x, interpClause i x = true
-                             -> exists l, In l x /\ interpLit i l = true.
-  induction x; simpl; try congruence; intros.
-  destruct (interpLit i a) eqn:?; eauto; simpl in *.
-  destruct IHx as [? [] ]; eauto.
-Qed.
-
-Lemma interpClause_In : forall l i x, interpLit i l = true -> In l x
-                                      -> interpClause i x = true.
-  induction x; simpl; try tauto; intros.
-  destruct H0; subst.
-  rewrite H; auto.
-  destruct (interpLit i a) eqn:?; eauto; simpl in *.
-Qed.
-
-Lemma interpClause_In' : forall x i l, interpClause i x = false
-                           -> In l x -> interpLit i l = false.
-  induction x; simpl; try tauto; intros.
-  eapply Bool.orb_false_iff in H; destruct H.
-  destruct H0; subst; auto.
-Qed.
-
-Hint Resolve interpClause_In interpClause_In'.
-
-Lemma interpClause_sublist : forall i x y, interpClause i x = true
-                               -> sublist x y -> interpClause i y = true.
-  intros.
-  edestruct interpClause_exists as [? [] ]; try eassumption.
-  eapply interpClause_In; try eassumption.
-  eapply Forall_forall in H0; eassumption.
-Qed.
-
-Lemma interpClause_sublist' : forall i x y, interpClause i y = false
-                                -> sublist x y -> interpClause i x = false.
-  induction x; simpl; intros; auto.
-  apply Bool.orb_false_iff.
-  inversion_clear H0; eauto 4.
-Qed.
-
-Hint Resolve interpClause_sublist interpClause_sublist'.
-
-Lemma interpClause_app : forall i x y,
-                           interpClause i x = true \/ interpClause i y = true
-                           -> interpClause i (x ++ y) = true.
-  intros; unfold interpClause; rewrite fold_right_app.
-  destruct H.
-  {
-    destruct (fold_right (fun (l : lit) (b : bool) => (interpLit i l || b)%bool)
-                false y); simpl; auto.
-    induction x; simpl in *; auto.
-    destruct (interpLit i a); auto.
-  }
-  {
-    unfold interpClause in H; rewrite H.
-    induction x; simpl; auto.
-    destruct (interpLit i a); auto.
-  }
-Qed.
-  
-Lemma interpFormula_In : forall f i c, interpFormula i f = true
-                                  -> In c f -> interpClause i c = true.
-  induction f; simpl; try tauto; intros.
-  destruct H0; subst.
-  apply Bool.andb_true_iff in H; tauto.
-  apply Bool.andb_true_iff in H; destruct H; auto.
-Qed.
-Hint Resolve interpFormula_In.
-
-Corollary In_entails : forall f c, In c f -> entails f c.
-  unfold entails; intros; eauto 3.
-Qed.
-Hint Resolve In_entails.
-
-
-(*=============================================================================
- * dpll
- *===========================================================================*)
 
 Section dpll.
   Variable numVars : nat.
@@ -245,6 +69,10 @@ End dpll.
  *===========================================================================*)
 
 Example numVars := 4.
+
+Example c1 := pos 3 :: nil.
+Example c2 := neg 3 :: nil.
+
 Example f1 := (@nil clause).
 Example f2 := c1 :: nil.
 Example f3 := c2 :: nil.
@@ -254,20 +82,75 @@ Eval compute in dpll numVars f3.
 
 
 (*=============================================================================
+ * semantics
+ *===========================================================================*)
+
+Definition interp := nat -> bool.
+
+Definition interpLit (I : interp) (l : lit) :=
+  match l with
+    | pos n => I n
+    | neg n => negb (I n)
+  end.
+
+Definition interpClause (I : interp) (c : clause) :=
+  fold_right (fun l b => orb (interpLit I l) b) false c.
+
+Definition interpFormula (I : interp) (f : formula) :=
+  fold_right (fun c b => andb (interpClause I c) b) true f.
+
+Definition satisfiable f := exists i, interpFormula i f = true.
+
+Definition entails f c := forall i, interpFormula i f = true
+                                    -> interpClause i c = true.
+
+
+(*=============================================================================
+ * semantics tests
+ *===========================================================================*)
+
+Example I n := match n with 0 => false | 1 => true | _ => true end.
+Eval simpl in interpLit I (pos 0).
+
+Goal forall (i : interp), interpClause i nil = false.
+  simpl; auto.
+Qed.
+
+Goal forall (i : interp), interpFormula i nil = true.
+  simpl; auto.
+Qed.
+
+Goal forall (i : interp) v, interpClause i ((pos v) :: (neg v) :: nil) = true.
+  simpl; intros.
+  destruct (i v) eqn:?; simpl; auto.
+Qed.
+
+Goal forall (i : interp), interpFormula i (c1 :: c2 :: nil) = false.
+  simpl; intros.
+  destruct (i 3) eqn:?; simpl; auto.
+Qed.
+
+
+(*=============================================================================
  * well-formedness of formula
  *===========================================================================*)
 
 Definition wf_clause nv c := forall l, In l c -> litVar l < nv.
 Definition wf_formula nv f := forall c, In c f -> wf_clause nv c.
 
+
+(*=============================================================================
+ * well-formedness tests
+ *===========================================================================*)
+
 Ltac wf :=
   unfold wf_formula; simpl; intros;
   repeat match goal with
            | _ => progress (subst; simpl)
-           | |- wf_clause _ ?c => progress unfold c; red; intros
+           | |- wf_clause _ ?c => try unfold c; red; intros
            | H: _ \/ _ |- _ => destruct H
            | H: In _ _ |- _ => inversion_clear H
-           | _ => tauto || solve [auto]
+           | _ => tauto || omega || solve [auto]
          end.
 
 Example f1_wf : wf_formula numVars f1.
@@ -319,7 +202,57 @@ Hint Resolve wf_formula_cons_inv'.
 (*=============================================================================
  * dpll correctness (SAT case)
  *===========================================================================*)
-Require Import Omega.
+
+Lemma getVal_Some : forall m n, n < length m -> getVal m n = Some (nth n m true).
+  induction m; simpl; intros; try omega.
+  destruct n; auto.
+  apply IHm; omega.
+Qed.
+
+Lemma getVal_None : forall n m, length m <= n -> getVal m n = None.
+  induction n; destruct m; simpl; auto; try omega; intros.
+  apply IHn; omega.
+Qed.
+
+Definition m2i m n := nth n m true.
+
+Lemma getVal_m2i : forall m n, n < length m -> getVal m n = Some (m2i m n).
+  unfold m2i; apply getVal_Some; auto.
+Qed.
+
+Lemma okLit_interpLit : forall m a, okLit m a = true -> litVar a < length m
+                                    -> interpLit (m2i m) a = true.
+  unfold okLit, interpLit; intros.
+  rewrite getVal_m2i in * by auto.
+  destruct a; simpl in *; auto.
+Qed.
+Hint Resolve okLit_interpLit.
+
+Lemma okClause_interpClause : forall nv m c, okClause m c = true
+                                  -> length m >= nv -> wf_clause nv c
+                                  -> interpClause (m2i m) c = true.
+  induction c; simpl; intros; try congruence.
+  apply Bool.orb_true_iff.
+  destruct (okLit m a) eqn:?; subst.
+  {
+    left; apply okLit_interpLit; auto.
+    assert (litVar a < nv) by (apply H1; simpl; auto).
+    omega.
+  }
+  {
+    right.
+    apply IHc; eauto 3.
+  }
+Qed.
+Hint Resolve okClause_interpClause.
+
+Lemma okFormula_interpFormula : forall nv m F, okFormula m F = true
+                                    -> length m >= nv -> wf_formula nv F
+                                    -> interpFormula (m2i m) F = true.
+  induction F; simpl; auto; intros.
+  destruct (okClause m a) eqn:?; try congruence.
+  apply Bool.andb_true_iff; split; eauto 3.
+Qed.
 
 Ltac dpll :=
   try match goal with
@@ -364,97 +297,12 @@ Theorem dpll_length : forall F nv m , dpll nv F = Some m
 Qed.
 Hint Resolve dpll_length.
 
-Lemma getVal_nth : forall m n, n < length m -> getVal m n = Some (nth n m true).
-  induction m; simpl; intros; try omega.
-  destruct n; auto.
-  apply IHm; omega.
-Qed.
-
-Definition m2i m n := nth n m true.
-
-Lemma getVal_m2i : forall m n, n < length m -> getVal m n = Some (m2i m n).
-  unfold m2i; apply getVal_nth; auto.
-Qed.
-
-Lemma okLit_interpLit : forall m a, okLit m a = true -> litVar a < length m
-                 -> interpLit (m2i m) a = true.
-  unfold okLit, interpLit; intros.
-  rewrite getVal_m2i in * by auto.
-  destruct a; simpl in *; auto.
-Qed.
-Hint Resolve okLit_interpLit.
-
-Lemma okClause_interpClause : forall nv m c, okClause m c = true
-                                  -> length m = nv -> wf_clause nv c
-                                  -> interpClause (m2i m) c = true.
-  induction c; simpl; intros; try congruence.
-  apply Bool.orb_true_iff.
-  destruct (okLit m a) eqn:?; subst.
-  {
-    left; apply okLit_interpLit; auto.
-    apply H1; simpl; auto.
-  }
-  {
-    right.
-    apply IHc; eauto 3.
-  }
-Qed.
-Hint Resolve okClause_interpClause.
-
-Lemma okFormula_interpFormula : forall nv m F, okFormula m F = true
-                                    -> length m = nv -> wf_formula nv F
-                                    -> interpFormula (m2i m) F = true.
-  induction F; simpl; auto; intros.
-  destruct (okClause m a) eqn:?; try congruence.
-  apply Bool.andb_true_iff; split; eauto 3.
-Qed.
-
 Theorem dpll_Some_sound : forall F m nv, dpll nv F = Some m -> wf_formula nv F
                                          -> satisfiable F.
   red; intros.
-  exists (m2i m); eapply okFormula_interpFormula; try eassumption; eauto 3.
+  assert (length m = nv) by eauto 3.
+  exists (m2i m); eapply okFormula_interpFormula; try eassumption; eauto 3; omega.
 Qed.
-
-
-(*=============================================================================
- * maxVarsFormula and well-formedness
- *===========================================================================*)
-
-Fixpoint maxVarsClause c :=
-  match c with
-    | nil => 0
-    | l :: c' => max (litVar l) (maxVarsClause c')
-  end.
-
-Fixpoint maxVarsFormula F :=
-  match F with
-    | nil => 0
-    | c :: F' => max (maxVarsClause c) (maxVarsFormula F')
-  end.
-
-Lemma maxVarsClause_wf_clause : forall n x, maxVarsClause x < n -> wf_clause n x.
-  induction x; simpl; red; simpl; try tauto; intros.
-  apply NPeano.Nat.max_lub_lt_iff in H; destruct H.
-  destruct H0; subst; try tauto.
-  apply IHx; auto.
-Qed.
-Hint Resolve maxVarsClause_wf_clause.
-
-Lemma maxVarsFormula_In : forall F c n, maxVarsFormula F < n -> In c F
-                                            -> maxVarsClause c < n.
-  induction F; simpl; try tauto; destruct 2; subst;
-  apply NPeano.Nat.max_lub_lt_iff in H; destruct H; auto.
-Qed.
-Hint Resolve maxVarsFormula_In.
-
-Lemma maxVarsFormula_lt_wf : forall n F, maxVarsFormula F < n -> wf_formula n F.
-  red; intros; eauto 3.
-Qed.
-
-Theorem wf_maxVarsFormula : forall F, wf_formula (1 + maxVarsFormula F) F.
-  intros; apply maxVarsFormula_lt_wf; omega.
-Qed.
-Hint Resolve wf_maxVarsFormula.
 
 
 (*=============================================================================
@@ -561,25 +409,11 @@ Lemma satisfiable_model : forall nv F, wf_formula nv F -> satisfiable F
   assert (interpFormula (clamp x nv) F = true) by auto.
   destruct (clamp_m2i x nv) as [? [] ]; eauto 4.
 Qed.
-  
-Lemma satisfiable_model' : forall F, satisfiable F
-                             -> exists m, interpFormula (m2i m) F = true.
-  destruct 1.
-  assert (wf_formula (1 + maxVarsFormula F) F) by auto.
-  assert (interpFormula (clamp x (1 + maxVarsFormula F)) F = true) by auto.
-  destruct (clamp_m2i x (1 + maxVarsFormula F)) as [? [] ]; eauto 4.
-Qed.
 
 
 (*=============================================================================
  * dpll correctness (UNSAT case)
  *===========================================================================*)
-
-Lemma getVal_None : forall n m, length m <= n -> getVal m n = None.
-  induction n; destruct m; simpl; auto; try omega; intros.
-  apply IHn; omega.
-Qed.
-
 
 Lemma okLit_interpLit' : forall m x, okLit m x = false
                                      -> interpLit (m2i m) x = false.
@@ -613,7 +447,7 @@ Lemma okLit_app : forall b m x, okLit m x = false
   unfold okLit; simpl; intros.
   destruct (le_lt_dec (length m) (litVar x)).
   rewrite getVal_None in * by auto; congruence.
-  rewrite getVal_nth in * by (autorewrite with list; omega).
+  rewrite getVal_Some in * by (autorewrite with list; omega).
   destruct x; simpl in *; rewrite app_nth1 by auto; auto.
 Qed.
 Hint Resolve okLit_app.
@@ -684,6 +518,199 @@ Qed.
 
 
 (*=============================================================================
+ * maxVarsFormula and well-formedness
+ *===========================================================================*)
+
+Fixpoint maxVarsClause c :=
+  match c with
+    | nil => 0
+    | l :: c' => max (litVar l) (maxVarsClause c')
+  end.
+
+Fixpoint maxVarsFormula F :=
+  match F with
+    | nil => 0
+    | c :: F' => max (maxVarsClause c) (maxVarsFormula F')
+  end.
+
+Lemma maxVarsClause_wf_clause : forall n x, maxVarsClause x < n -> wf_clause n x.
+  induction x; simpl; red; simpl; try tauto; intros.
+  apply NPeano.Nat.max_lub_lt_iff in H; destruct H.
+  destruct H0; subst; try tauto.
+  apply IHx; auto.
+Qed.
+Hint Resolve maxVarsClause_wf_clause.
+
+Lemma maxVarsFormula_In : forall F c n, maxVarsFormula F < n -> In c F
+                                            -> maxVarsClause c < n.
+  induction F; simpl; try tauto; destruct 2; subst;
+  apply NPeano.Nat.max_lub_lt_iff in H; destruct H; auto.
+Qed.
+Hint Resolve maxVarsFormula_In.
+
+Lemma maxVarsFormula_lt_wf : forall n F, maxVarsFormula F < n -> wf_formula n F.
+  red; intros; eauto 3.
+Qed.
+
+Theorem wf_maxVarsFormula : forall F, wf_formula (1 + maxVarsFormula F) F.
+  intros; apply maxVarsFormula_lt_wf; omega.
+Qed.
+Hint Resolve wf_maxVarsFormula.
+
+
+(*=============================================================================
+ * conjecture : stronger theorem
+ *===========================================================================*)
+
+Conjecture conj : forall F n, dpll n F = None
+                              -> dpll (1 + maxVarsFormula F) F = None.
+
+Lemma satisfiable_model' : forall F, satisfiable F
+                             -> exists m, interpFormula (m2i m) F = true
+                                          /\ length m = 1 + maxVarsFormula F.
+  destruct 1.
+  assert (wf_formula (1 + maxVarsFormula F) F) by auto.
+  assert (interpFormula (clamp x (1 + maxVarsFormula F)) F = true) by auto.
+  destruct (clamp_m2i x (1 + maxVarsFormula F)) as [? [] ]; eauto 4.
+Qed.
+
+Theorem dpll_None_sound' : forall n F, dpll n F = None
+                                       -> ~ satisfiable F.
+  red; intros.
+  assert (dpll (1 + maxVarsFormula F) F = None).
+  solve [eapply conj; eauto 3].
+  edestruct satisfiable_model' as [? [] ]; eauto 3.
+  assert (wf_formula (1 + maxVarsFormula F) F) by auto.
+  assert (interpFormula (m2i x) F = false).
+  solve [eapply dpll_None'; eauto 3].
+  congruence.
+Qed.
+
+
+(*=============================================================================
+ * sublist
+ *===========================================================================*)
+
+Section sublist.
+
+  Ltac e := eauto 3 with list.
+
+  Local Hint Constructors Forall : list.
+  Local Hint Resolve in_or_app Forall_impl : list.
+
+  Variable A : Type.
+
+  Definition sublist (x y : list A) := List.Forall (fun a => In a y) x.
+
+  Lemma sublist_refl : forall (x : list A), sublist x x.
+    unfold sublist; induction x; e.
+    constructor; simpl; e.
+    eapply Forall_impl; try eassumption; e.
+  Qed.
+
+  Lemma sublist_app : forall (l x y : list A), sublist l x \/ sublist l y
+                                                 -> sublist l (x ++ y).
+    induction l.
+    {
+      unfold sublist; simpl; intros; e.
+    }
+    {
+      unfold sublist; simpl; intros.
+      constructor.
+      destruct H; inversion_clear H; e.
+      apply IHl.
+      destruct H; inversion_clear H; e.
+    }
+  Qed.
+
+  Lemma sublist_In : forall x (a : A) y, sublist x y -> In a x -> In a y.
+    induction x; simpl; try tauto; inversion_clear 1; destruct 1; subst; auto.
+  Qed.
+
+End sublist.
+
+Local Hint Resolve sublist_refl sublist_app sublist_In.
+
+
+(*=============================================================================
+ * interp facts
+ *===========================================================================*)
+
+Lemma interpClause_exists : forall i x, interpClause i x = true
+                             -> exists l, In l x /\ interpLit i l = true.
+  induction x; simpl; try congruence; intros.
+  destruct (interpLit i a) eqn:?; eauto; simpl in *.
+  destruct IHx as [? [] ]; eauto.
+Qed.
+
+Lemma interpClause_In : forall l i x, interpLit i l = true -> In l x
+                                      -> interpClause i x = true.
+  induction x; simpl; try tauto; intros.
+  destruct H0; subst.
+  rewrite H; auto.
+  destruct (interpLit i a) eqn:?; eauto; simpl in *.
+Qed.
+
+Lemma interpClause_In' : forall x i l, interpClause i x = false
+                           -> In l x -> interpLit i l = false.
+  induction x; simpl; try tauto; intros.
+  eapply Bool.orb_false_iff in H; destruct H.
+  destruct H0; subst; auto.
+Qed.
+
+Hint Resolve interpClause_In interpClause_In'.
+
+Lemma interpClause_sublist : forall i x y, interpClause i x = true
+                               -> sublist x y -> interpClause i y = true.
+  intros.
+  edestruct interpClause_exists as [? [] ]; try eassumption.
+  eapply interpClause_In; try eassumption.
+  eapply Forall_forall in H0; eassumption.
+Qed.
+
+Lemma interpClause_sublist' : forall i x y, interpClause i y = false
+                                -> sublist x y -> interpClause i x = false.
+  induction x; simpl; intros; auto.
+  apply Bool.orb_false_iff.
+  inversion_clear H0; eauto 4.
+Qed.
+
+Hint Resolve interpClause_sublist interpClause_sublist'.
+
+Lemma interpClause_app : forall i x y,
+                           interpClause i x = true \/ interpClause i y = true
+                           -> interpClause i (x ++ y) = true.
+  intros; unfold interpClause; rewrite fold_right_app.
+  destruct H.
+  {
+    destruct (fold_right (fun (l : lit) (b : bool) => (interpLit i l || b)%bool)
+                false y); simpl; auto.
+    induction x; simpl in *; auto.
+    destruct (interpLit i a); auto.
+  }
+  {
+    unfold interpClause in H; rewrite H.
+    induction x; simpl; auto.
+    destruct (interpLit i a); auto.
+  }
+Qed.
+  
+Lemma interpFormula_In : forall f i c, interpFormula i f = true
+                                  -> In c f -> interpClause i c = true.
+  induction f; simpl; try tauto; intros.
+  destruct H0; subst.
+  apply Bool.andb_true_iff in H; tauto.
+  apply Bool.andb_true_iff in H; destruct H; auto.
+Qed.
+Hint Resolve interpFormula_In.
+
+Corollary In_entails : forall f c, In c f -> entails f c.
+  unfold entails; intros; eauto 3.
+Qed.
+Hint Resolve In_entails.
+
+
+(*=============================================================================
  * resolvent
  *===========================================================================*)
 
@@ -738,7 +765,7 @@ Hint Resolve resolvent_entails.
 
 
 (*=============================================================================
- * resolution (direct)
+ * Example : (direct) resolution
  *===========================================================================*)
 
 Definition resolve x y v := remove_lit (pos v) x ++ remove_lit (neg v) y.
@@ -776,7 +803,7 @@ Lemma pf_nil_interp_false : forall f, pf f nil
   simpl in *; congruence.
 Qed.
 
-Theorem pf_nil_unsat : forall f, pf f nil -> ~ satisfiable f.
+Lemma pf_nil_unsat : forall f, pf f nil -> ~ satisfiable f.
   intros; red; destruct 1.
   assert (interpFormula x f = false).
   solve [apply pf_nil_interp_false; auto].
@@ -788,6 +815,20 @@ Qed.
  * todo: pf is refutation complete
  *===========================================================================*)
 
+Conjecture pf_complete : forall f, entails f nil -> pf f nil.
+
+Lemma unsat_pf_nil : forall f, ~ satisfiable f -> pf f nil.
+  intros; apply pf_complete.
+  red; intros.
+  contradict H.
+  red; eauto.
+Qed.
+  
+Theorem dpll_pf : forall n F, wf_formula n F -> dpll n F = None -> pf F nil.
+  intros; apply unsat_pf_nil.
+  eapply dpll_None_sound; eauto 2.
+Qed.
+  
 
 (*=============================================================================
  * denotation into Coq
@@ -872,3 +913,214 @@ Lemma pf_denote_sound : forall f g c, pf f c -> denoteFormula g f
                                       -> denoteClause g c.
   induction 1; intros; eauto 4.
 Qed.
+
+
+(*=============================================================================
+ * trimmed denotation
+ *===========================================================================*)
+
+Fixpoint denoteClause' (g : context) (c : clause) : Prop :=
+  match c with
+    | nil => False
+    | l :: nil => denoteLit g l
+    | l :: c' => denoteLit g l \/ denoteClause' g c'
+  end.
+
+Fixpoint denoteFormula' (g : context) f : Prop :=
+  match f with
+    | nil => True
+    | c :: nil => denoteClause' g c
+    | c :: f' => denoteClause' g c /\ denoteFormula' g f'
+  end.
+
+Lemma denoteClause_trim : forall g c, denoteClause' g c -> denoteClause g c.
+  induction c; simpl; try tauto; intros.
+  destruct c; auto; simpl in *; tauto.
+Qed.
+Hint Resolve denoteClause_trim.
+
+Lemma denoteFormula_trim : forall g x, denoteFormula' g x -> denoteFormula g x.
+  induction x; simpl; try tauto; intros.
+  destruct x; simpl; auto.
+  destruct H.
+  split; auto.
+  apply IHx; auto.
+Qed.
+Hint Resolve denoteFormula_trim.
+
+Lemma denoteClause_trim' : forall g c, denoteClause g c -> denoteClause' g c.
+  induction c; simpl; try tauto; intros.
+  destruct H, c; auto; simpl in *; tauto.
+Qed.
+
+Lemma pf_denote_sound' : forall f g c, pf f c -> denoteFormula' g f
+                                       -> denoteClause' g c.
+  intros.
+  apply denoteClause_trim'.
+  eapply pf_denote_sound; eauto 3.
+Qed.
+
+
+(*=============================================================================
+ * reification
+ *===========================================================================*)
+
+Ltac inList x xs :=
+  match xs with
+    | nil => false
+    | x :: _ => true
+    | _ :: ?xs' => inList x xs'
+  end.
+
+Ltac addToList x xs :=
+  let b := inList x xs in
+  match b with
+    | true => xs
+    | false => constr:(x :: xs)
+  end.
+
+Ltac lookup x xs :=
+  match xs with
+    | x :: _ => constr:O
+    | _ :: ?xs' => let n := lookup x xs' in constr:(S n)
+  end.
+
+
+Ltac allVars xs e :=
+  match e with
+    | ~ ?e' => allVars xs e'
+    | ?e1 /\ ?e2 => let xs := allVars xs e1 in allVars xs e2
+    | ?e1 \/ ?e2 => let xs := allVars xs e1 in allVars xs e2
+    | _ => addToList e xs
+  end.
+
+Ltac reifyLit g e :=
+  match e with
+    | not ?e' => let v := lookup e' g in constr:(neg v)
+    | _ => let v := lookup e g in constr:(pos v)
+  end.
+
+Ltac reifyClause g e :=
+  match e with
+    | ?x \/ ?y =>
+      let l := reifyLit g x in
+      let c := reifyClause g y in
+      constr:(l :: c)
+    | _ =>
+      let l := reifyLit g e in
+      constr:(l :: nil)
+  end.
+
+Ltac reifyFormula g e :=
+  match e with
+    | ?x /\ ?y =>
+      let c := reifyClause g x in
+      let f := reifyFormula g y in
+      constr:(c :: f)
+    | _ =>
+      let c := reifyClause g e in
+      constr:(c :: nil)
+  end.
+
+Ltac reify :=
+  match goal with
+    | |- ?F =>
+      let g := allVars tt F in
+      let f := reifyFormula g F in
+      pose f
+  end.
+
+
+(*=============================================================================
+ * reification tests
+ *===========================================================================*)
+
+Section reification_test.
+  Variables A B C D : Prop.
+
+  Goal (A /\ ~ B) -> A.
+    match goal with
+      | |- ?F -> ?C =>
+        let _g := allVars (@nil Prop) F in
+        let _f := reifyFormula _g F in
+        let _c := reifyClause _g C in
+        pose (g:=_g); pose (f:=_f); pose (c:=_c)
+    end.
+    intro.
+    change (denoteFormula' g f) in H.
+    change (denoteClause' g c).
+    eapply pf_denote_sound'; eauto 3.
+    {
+      constructor; wf.
+    }
+  Qed.
+End reification_test.
+
+
+(*=============================================================================
+ * reflection tests
+ *===========================================================================*)
+
+Section PigeonHole.
+  Variables p1 p2 p3 p4 p5 p6 p7 p8 p9 p10 p11 p12 : Prop.
+
+  Definition hole2 :=
+    (~p1 \/ ~p3) /\
+    (~p1 \/ ~p5) /\
+    (~p3 \/ ~p5) /\
+    (~p2 \/ ~p4) /\
+    (~p2 \/ ~p6) /\
+    (~p4 \/ ~p6) /\
+    (p1 \/ p2) /\
+    (p3 \/ p4) /\
+    (p5 \/ p6).
+
+  Definition hole3 :=
+    (~p1 \/ ~p4) /\
+    (~p1 \/ ~p7) /\
+    (~p1 \/ ~p10) /\
+    (~p4 \/ ~p7) /\
+    (~p4 \/ ~p10) /\
+    (~p7 \/ ~p10) /\
+
+    (~p2 \/ ~p5) /\
+    (~p2 \/ ~p8) /\
+    (~p2 \/ ~p11) /\
+    (~p5 \/ ~p8) /\
+    (~p5 \/ ~p11) /\
+    (~p8 \/ ~p11) /\
+
+    (~p3 \/ ~p6) /\
+    (~p3 \/ ~p9) /\
+    (~p3 \/ ~p12) /\
+    (~p6 \/ ~p9) /\
+    (~p6 \/ ~p12) /\
+    (~p9 \/ ~p12) /\
+
+    (p1 \/ p2 \/ p3) /\
+    (p4 \/ p5 \/ p6) /\
+    (p7 \/ p8 \/ p9) /\
+    (p10 \/ p11 \/ p12).
+
+  (*Goal hole2 -> False.
+    unfold hole2; tauto.
+  Qed.*)
+
+  Goal hole3 -> False. (* tauto will be very slow *)
+    unfold hole3.
+    match goal with
+      | |- ?F -> False =>
+        let _g := allVars (@nil Prop) F in
+        let _f := reifyFormula _g F in
+        pose (g:=_g); pose (f:=_f)
+    end.
+    intro H.
+    change (denoteFormula' g f) in H.
+    change (denoteClause' g nil).
+    eapply pf_denote_sound'; eauto 3.
+    assert (wf_formula 12 f) by wf.
+    eapply dpll_pf; try eassumption.
+    compute; auto.
+  Qed.
+
+End PigeonHole.
